fix proofs

theories/typing/uniq_bor.v
@@ -1,5 +1,5 @@
 From lrust.typing Require Export type.
-From lrust.typing Require Import type_context programs mod_ty.
+From lrust.typing Require Import type_context programs mod_ty uniq_util.
 Set Default Proof Using "Type".
 
 Implicit Type 𝔄 𝔅: syn_type.
@@ -7,20 +7,28 @@ Implicit Type 𝔄 𝔅: syn_type.
 Section uniq_bor.
   Context `{!typeG Σ}.
 
-  Definition prval_to_inh' {𝔄} (vπ: proph (𝔄 * 𝔄))
-    : inh_syn_type 𝔄 := prval_to_inh (fst ∘ vπ).
+  Lemma split_mt_uniq_bor l' P Φ Ψ :
+    (l' ↦∗: (λ vl, P ∗ [loc[l] := vl]
+      ∃(d: nat) (ξi: positive), ⌜Ψ d ξi⌝ ∗ Φ l d ξi)) ⊣⊢
+    P ∗ ∃(l: loc) d ξi, ⌜Ψ d ξi⌝ ∗ l' ↦ #l ∗ Φ l d ξi.
+  Proof.
+    iSplit.
+    - iDestruct 1 as ([|[[]|][]]) "(↦ &$& big)"=>//. iDestruct "big" as (???) "?".
+      iExists _, _, _. rewrite heap_mapsto_vec_singleton. by iFrame.
+    - iIntros "($&%&%&%&%& ↦ &?)". iExists [_]. rewrite heap_mapsto_vec_singleton.
+      iFrame "↦". iExists _, _. by iFrame.
+  Qed.
 
   Program Definition uniq_bor {𝔄} (κ: lft) (ty: type 𝔄) : type (𝔄 * 𝔄) := {|
     ty_size := 1;  ty_lfts := κ :: ty.(ty_lfts);  ty_E := ty.(ty_E) ++ ty_outlives_E ty κ;
-    ty_own vπ d tid vl := κ ⊑ ty.(ty_lft) ∗ [loc[l] := vl] ∃d' i,
-      let ξ := PrVar (𝔄 ↾ prval_to_inh' vπ) i in
-      ⌜(S d' ≤ d)%nat ∧ snd ∘ vπ = (.$ ξ)⌝ ∗ .VO[ξ] (fst ∘ vπ) d' ∗
-      &{κ} (∃vπ' d', ⧖(S d') ∗ .PC[ξ] vπ' d' ∗ l ↦∗: ty.(ty_own) vπ' d' tid);
+    ty_own vπ d tid vl := κ ⊑ ty.(ty_lft) ∗ [loc[l] := vl] ∃d' ξi,
+      let ξ := PrVar (𝔄 ↾ prval_to_inh (fst ∘ vπ)) ξi in
+      ⌜(S d' ≤ d)%nat ∧ snd ∘ vπ = (.$ ξ)⌝ ∗ uniq_own ty (fst ∘ vπ) ξi d' κ tid l;
     ty_shr vπ d κ' tid l := [S(d') := d] ∃(l': loc) ξ, ⌜snd ∘ vπ ./ [ξ]⌝ ∗
-      &frac{κ'} (λ q', l ↦{q'} #l') ∗ &frac{κ'} (λ q, q:[ξ]) ∗
+      &frac{κ'} (λ q, l ↦{q} #l') ∗ &frac{κ'} (λ q, q:[ξ]) ∗
       ▷ ty.(ty_shr) (fst ∘ vπ) d' κ' tid l';
   |}%I.
-  Next Obligation. move=>/= *. rewrite by_just_loc_ex. by iIntros "[_ [%[->?]]]".  Qed.
+  Next Obligation. move=>/= *. rewrite by_just_loc_ex. by iIntros "[_ [%[->?]]]". Qed.
   Next Obligation. move=>/= > H. by setoid_rewrite H. Qed.
   Next Obligation.
     move=> ???[|?][|?]*/=; try (by iIntros); [lia|]. do 8 f_equiv.
@@ -32,65 +40,34 @@ Section uniq_bor.
     by iApply ty_shr_lft_mono.
   Qed.
   Next Obligation.
-    move=> 𝔄 ??? vπ *. have ?: Inhabited 𝔄 := populate (vπ inhabitant).1.
-    iIntros "#LFT #? Bor κ'". iMod (bor_exists with "LFT Bor") as (vl) "Bor"; [done|].
+    move=> 𝔄 ??? vπ d *. have ?: Inhabited 𝔄 := populate (vπ inhabitant).1.
+    iIntros "#LFT #? Bor κ'". rewrite split_mt_uniq_bor.
+    iMod (bor_sep with "LFT Bor") as "[_ Bor]"; [done|].
+    do 3 (iMod (bor_exists with "LFT Bor") as (?) "Bor"; [done|]).
+    iMod (bor_sep_persistent with "LFT Bor κ'") as "(>[%->] & Bor & κ')"; [done|].
+    case d as [|]; [lia|]. iApply step_fupdN_nmono; [done|].
     iMod (bor_sep with "LFT Bor") as "[Bor↦ Bor]"; [done|].
-    iMod (bor_sep with "LFT Bor") as "[_ Bor]"; [done|].
-    rewrite by_just_loc_ex. iMod (bor_exists with "LFT Bor") as (l) "Bor"; [done|].
-    iMod (bor_sep_persistent with "LFT Bor κ'") as "(>->& Bor & κ')"; [done|].
-    iMod (bor_exists with "LFT Bor") as (?) "Bor"; [done|].
-    iMod (bor_exists with "LFT Bor") as (i) "Bor"; [done|].
-    set ξ := PrVar (𝔄 ↾ prval_to_inh' vπ) i.
-    iMod (bor_sep_persistent with "LFT Bor κ'") as
-    "(>%H & Bor & κ')"; [done|]. move: H=> [/succ_le [d[->Le]]->]/=.
-    iMod (bor_sep with "LFT Bor") as "[BorVo Bor]"; [done|].
-    iMod (bor_unnest with "LFT Bor") as "Bor"; [done|]. iIntros "!>!>!>".
-    iMod (bor_shorten with "[] Bor") as "Bor".
-    { iApply lft_incl_glb; [|iApply lft_incl_refl].
-      iApply lft_incl_trans; by [|iApply lft_intersect_incl_l]. }
-    do 2 (iMod (bor_exists with "LFT Bor") as (?) "Bor"; [done|]).
-    iMod (bor_sep with "LFT Bor") as "[_ Bor]"; [done|].
-    iMod (bor_sep with "LFT Bor") as "[BorPc Borty]"; [done|].
-    iMod (bor_combine with "LFT BorVo BorPc") as "Bor"; [done|].
-    iMod (bor_acc_cons with "LFT Bor κ'") as "[[Vo Pc] ToBor]"; [done|].
-    iMod (uniq_strip_later with "Vo Pc") as (->->) "[Vo Pc]".
-    iDestruct (uniq_proph_tok with "Vo Pc") as "(Vo & ξ & ToPc)".
-    iMod ("ToBor" with "[Vo ToPc] ξ") as "[Borξ κ']".
-    { iIntros "!> >ξ !>!>". iFrame "Vo". by iApply "ToPc". }
-    iMod (ty_share with "LFT [] Borty κ'") as "Upd"; [done| |].
-    { iApply lft_incl_trans; by [|iApply lft_intersect_incl_r]. }
-    iApply step_fupdN_nmono; [by apply Le|]. iApply (step_fupdN_wand with "Upd").
-    rewrite heap_mapsto_vec_singleton.
     iMod (bor_fracture (λ q, _ ↦{q} _)%I with "LFT Bor↦") as "Bor↦"; [done|].
-    iMod (bor_fracture (λ q, q:[_])%I with "LFT Borξ") as "Borξ"; [done|].
-    iIntros "!> >[?$] !>". iExists l, ξ. iFrame "Bor↦ Borξ".
-    iSplit; [iPureIntro; apply proph_dep_one|]. iApply ty_shr_depth_mono; by [|lia].
+    iMod (ty_share_uniq_own with "LFT [] [] Bor κ'") as "Upd"; [done|..].
+    { iApply lft_incl_trans; [done|]. iApply lft_intersect_incl_l. }
+    { iApply lft_incl_trans; [done|]. iApply lft_intersect_incl_r. }
+    iApply (step_fupdN_wand with "Upd").
+    iIntros "!> >(Borξ & ty &$) !>". iExists _, _. iFrame "Bor↦ Borξ".
+    iSplit; [iPureIntro; apply proph_dep_one|].
+    iApply ty_shr_depth_mono; [|done]. lia.
   Qed.
   Next Obligation.
-    move=> 𝔄 ??? vπ *. iIntros "#LFT #?". setoid_rewrite by_just_loc_ex at 1.
-    iIntros "[In (%&->& Big)]". iDestruct "Big" as (d i [Le Eq]) "[Vo Bor]".
-    set ξ := PrVar (𝔄 ↾ prval_to_inh' vπ) i. move: Le=> /succ_le [?[->Le]].
-    iIntros "[κ1 κ1₊]".
-    iMod (lft_incl_acc with "[] κ1") as (?) "[κ1 Toκ1]"; first done.
-    { iApply lft_incl_trans; by [|iApply lft_intersect_incl_l]. }
-    iMod (bor_acc with "LFT Bor κ1") as "[Big ToBor]"; [done|]. iIntros "!>!>!>".
-    iDestruct "Big" as (??) "(#⧖ & Pc & %vl & ↦ & ty)".
-    iDestruct (uniq_agree with "Vo Pc") as %[<-<-].
-    iDestruct (uniq_proph_tok with "Vo Pc") as "(Vo & ξ & ToPc)".
-    iMod (ty_own_proph with "LFT [] ty κ1₊") as "Upd"; [done| |].
-    { iApply lft_incl_trans; by [|iApply lft_intersect_incl_r]. }
-    iModIntro. iApply step_fupdN_nmono; [by apply Le|].
-    iApply (step_fupdN_wand with "Upd"). iMod 1 as (ζl ??) "[ζl Toty]". iModIntro.
-    rewrite proph_tok_singleton.
-    iDestruct (proph_tok_combine with "ζl ξ") as (q) "[ζlξ Toζlξ]".
-    iExists (ζl ++ [ξ]), q. iSplit.
+    move=> 𝔄 *. iIntros "#LFT #?". setoid_rewrite by_just_loc_ex at 1.
+    iIntros "[$ (%&->& Big)] κ'". iDestruct "Big" as (? ξi [Le Eq]) "uniq".
+    iMod (ty_own_proph_uniq_own with "LFT [] [] uniq κ'") as "Upd"; [done|..].
+    { iApply lft_incl_trans; [done|]. iApply lft_intersect_incl_l. }
+    { iApply lft_incl_trans; [done|]. iApply lft_intersect_incl_r. }
+    iApply step_fupdN_nmono; [by apply Le|]. iApply (step_fupdN_wand with "Upd").
+    iIntros "!> >(%&%&%& [ζlξ Touniq]) !>".
+    set ξ := PrVar _ ξi. iExists (_++[ξ]), _. iSplit.
     { iPureIntro. apply proph_dep_pair; [done|]. rewrite Eq. apply proph_dep_one. }
-    iIntros "{$ζlξ}ζlξ". iDestruct ("Toζlξ" with "ζlξ") as "[ζl ξ]".
-    iMod ("Toty" with "ζl") as "[ty $]". iDestruct ("ToPc" with "ξ") as "Pc".
-    iMod ("ToBor" with "[Pc ↦ ty]") as "[Bor κ1]".
-    { iModIntro. iExists (fst ∘ vπ), d. iFrame "Pc ⧖". iExists vl. iFrame. }
-    iMod ("Toκ1" with "κ1") as "$". iModIntro. iFrame "In". iExists d, i.
-    iFrame "Vo Bor". iPureIntro. split; [lia|done].
+    iIntros "{$ζlξ}ζlξ". iMod ("Touniq" with "ζlξ") as "[uniq $]". iModIntro.
+    iExists _, _. by iFrame.
   Qed.
   Next Obligation.
     move=> ?????[|?]*; [by iIntros|].
@@ -110,7 +87,7 @@ Section uniq_bor.
   Qed.
 
   Global Instance uniq_bor_ne {𝔄} κ : NonExpansive (@uniq_bor 𝔄 κ).
-  Proof. solve_ne_type. Qed.
+  Proof. rewrite /uniq_bor /uniq_own. solve_ne_type. Qed.
 End uniq_bor.
 
 Notation "&uniq{ κ }" := (uniq_bor κ) (format "&uniq{ κ }") : lrust_type_scope.
@@ -124,12 +101,12 @@ Section typing.
     - move=> > ? Hl * /=. f_equiv.
       + apply equiv_dist. iDestruct Hl as "#[??]".
         iSplit; iIntros "#H"; (iApply lft_incl_trans; [iApply "H"|done]).
-      + do 18 (f_contractive || f_equiv). by simpl in *.
+      + rewrite /uniq_own. do 18 (f_contractive || f_equiv). by simpl in *.
     - move=> */=. do 10 (f_contractive || f_equiv). by simpl in *.
   Qed.
 
   Global Instance uniq_send {𝔄} κ (ty: type 𝔄) : Send ty → Send (&uniq{κ} ty).
-  Proof. move=> >/=. by do 19 f_equiv. Qed.
+  Proof. move=> >/=. rewrite /uniq_own. by do 19 f_equiv. Qed.
 
   Global Instance uniq_sync {𝔄} κ (ty: type 𝔄) : Sync ty → Sync (&uniq{κ} ty).
   Proof. move=> >/=. by do 10 f_equiv. Qed.
@@ -140,21 +117,11 @@ Section typing.
   Lemma uniq_leak {𝔄} E L κ (ty: type 𝔄) :
     lctx_lft_alive E L κ → leak E L (&uniq{κ} ty) (λ '(a, a'), a' = a).
   Proof.
-    move=>/= Alv ?? vπ d ? vl ?. iIntros "#LFT PROPH E L [In uniq]".
-    case vl as [|[[]|][]]=>//. iDestruct "uniq" as (??[Le Eq]) "[Vo Bor]".
-    move: Le=> /succ_le[?[->Le]]/=.
-    have ?: Inhabited 𝔄 := populate (vπ inhabitant).1.
-    iMod (Alv with "E L") as (?) "[[κ κ₊] ToL]"; [solve_ndisj|].
-    iMod (bor_acc with "LFT Bor κ") as "[(%&%& ⧖ & Pc &%& ↦ & ty) ToBor]";
-      [solve_ndisj|]. iIntros "!>!>!>".
-    iMod (ty_own_proph with "LFT In ty κ₊") as "Toξl"; [solve_ndisj|].
-    iDestruct (uniq_agree with "Vo Pc") as %[<-->].
-    iApply step_fupdN_nmono; [by apply Le|].
-    iApply (step_fupdN_wand with "Toξl"). iIntros "!> >(%&%&%& ξl & Toty)".
-    iMod (uniq_resolve with "PROPH Vo Pc ξl") as "(Obs & Pc & ξl)"; [solve_ndisj|done|].
-    iMod ("Toty" with "ξl") as "[ty κ₊]". iMod ("ToBor" with "[⧖ Pc ↦ ty]") as "[_ κ]".
-    { iNext. iExists _, _. iFrame "⧖ Pc". iExists _. iFrame. }
-    iSplitL "Obs"; [|iApply "ToL"; by iFrame]. iApply proph_obs_eq; [|done]=>/= π.
+    move=>/= ??? vπ ?? vl ?. iIntros "LFT PROPH E L [In uniq]".
+    case vl as [|[[]|][]]=>//. iDestruct "uniq" as (??[Le Eq]) "uniq".
+    iMod (leak_uniq_own with "LFT PROPH In E L uniq") as "Upd"; [done..|].
+    iApply step_fupdN_nmono; [done|]. iApply (step_fupdN_wand with "Upd").
+    iIntros "!> >(?&$) !>". iApply proph_obs_eq; [|done]=>/= π.
     move: (equal_f Eq π)=>/=. by case (vπ π)=>/= ??->.
   Qed.
 
@@ -163,19 +130,11 @@ Section typing.
     real E L (&uniq{κ} ty) (f ∘ fst).
   Proof.
     move=> Alv [Rlo Rls]. split.
-    - iIntros (????? [|[[]|][]] ?) "#LFT #E [L L₊] [$ uniq] //".
-      iDestruct "uniq" as (d' ?[Le Eq]) "[Vo Bor]".
-      move: Le=> /succ_le[?[-> Le]]/=.
-      iMod (Alv with "E L") as (?) "[κ ToL]"; [done|].
-      iMod (bor_acc with "LFT Bor κ") as "[big ToBor]"; [done|].
-      iIntros "!>!>!>". iDestruct "big" as (??) "(⧖' & Pc &%& ↦ & ty)".
-      iDestruct (uniq_agree with "Vo Pc") as %[<-<-].
-      iMod (Rlo with "LFT E L₊ ty") as "Upd"; [done|].
-      iApply step_fupdN_nmono; [by apply Le|]. iApply (step_fupdN_wand with "Upd").
-      iIntros "!> >($&$& ty)". iMod ("ToBor" with "[⧖' Pc ↦ ty]") as "[Bor κ]".
-      { iNext. iExists _, _. iFrame "⧖' Pc". iExists _. iFrame. }
-      iMod ("ToL" with "κ") as "$". iModIntro. iExists d', _. iFrame "Vo Bor".
-      iPureIntro. split; [lia|done].
+    - iIntros (????? vl ?) "#LFT #E L [$ uniq]". case vl as [|[[]|][]]=>//.
+      iDestruct "uniq" as (d' ?[??]) "uniq". iApply step_fupdN_nmono; [done|].
+      iMod (real_uniq_own with "LFT E L uniq") as "Upd"; [done..|].
+      iApply (step_fupdN_wand with "Upd"). iIntros "!> >($&$& uniq) !>".
+      iExists _, _. by iFrame.
     - iIntros (???[|]????) "LFT E L uniq //".
       iDestruct "uniq" as (???) "(Bor & Bor' & ty)". iIntros "!>!>!>/=".
       iMod (Rls with "LFT E L ty") as "Upd"; [done|]. iIntros "!>!>".
@@ -193,10 +152,8 @@ Section typing.
     iSplit; iModIntro=>/=.
     - iIntros "*". rewrite {1}by_just_loc_ex. iIntros "[#? (%&->& Big)]".
       iSplitR. { iApply lft_incl_trans; [|done]. by iApply lft_incl_trans. }
-      iDestruct "Big" as (d' ξ ?) "[Vo ?]". iExists d', ξ. iSplit; [done|]. iFrame "Vo".
-      iApply (bor_shorten with "In"). iApply bor_iff; [|done]. iIntros "!>!>".
-      iSplit; iDestruct 1 as (vπ' d'') "(⧖ & Pc &%vl & ↦ & ?)"; iExists vπ', d'';
-      iFrame "⧖ Pc"; iExists vl; iFrame "↦"; by iApply "EqOwn".
+      iDestruct "Big" as (???) "uniq". iExists _, _. iSplit; [done|].
+      by iApply incl_uniq_own.
     - iIntros (?[|?]???); [by iIntros|]. iDestruct 1 as (l' ξ ?) "(?&?&?)".
       iExists l', ξ. do 3 (iSplit; [done|]). by iApply "EqShr".
   Qed.
@@ -209,20 +166,20 @@ Section typing.
     lctx_lft_alive E L κ →
     typed_write E L (&uniq{κ} ty) ty (&uniq{κ} ty) ty fst (λ v w, (w, v.2)).
   Proof.
-    move=> Alv. split; [done|]. iIntros (vπ d[[]|]??) "#LFT #UNIQ E L [In uniq] //".
-    have ?: Inhabited 𝔄 := populate (vπ inhabitant).1.
-    iDestruct "uniq" as (??[Le ?]) "[Vo Bor]". move: Le=> /succ_le[?[->?]].
+    move=> Alv. split; [done|]. iIntros (vπ d l ??) "#LFT #UNIQ E L [$ uniq]".
+    case l as [[]|]=>//. iDestruct "uniq" as (? ξi [??]) "[Vo Bor]".
     iMod (Alv with "E L") as (?) "[κ ToL]"; [done|].
     iMod (bor_acc with "LFT Bor κ") as "[(%&%&_& Pc &%& >↦ & ty) ToBor]"; [done|].
     iMod (uniq_strip_later with "Vo Pc") as (<-<-) "[Vo Pc]". iModIntro.
     iExists _. iSplit; [done|]. iSplitL "↦ ty".
     { iNext. iExists _. iFrame "↦". iApply ty_own_depth_mono; [|done]. lia. }
-    iIntros (wπ ?) "(% & >↦ & ty) #⧖ /=".
+    iIntros (wπ d'') "(% & >↦ & ty) #⧖ /=".
     iMod (uniq_update with "UNIQ Vo Pc") as "[Vo Pc]"; [done|].
     iMod ("ToBor" with "[↦ Pc ty]") as "[Bor κ]".
     { iNext. iExists _, _. iFrame "⧖ Pc". iExists _. iFrame. }
-    iMod ("ToL" with "κ") as "$". iFrame "In". iExists _, _.
-    rewrite (proof_irrel (prval_to_inh' _) (prval_to_inh' vπ)). by iFrame.
+    iMod ("ToL" with "κ") as "$". iModIntro. iExists d'', ξi.
+    rewrite /uniq_own (proof_irrel (prval_to_inh _) (prval_to_inh (fst ∘ vπ))).
+    by iFrame.
   Qed.
 
   Lemma read_uniq {𝔄} E L κ (ty: type 𝔄):
@@ -242,77 +199,6 @@ Section typing.
     iIntros "↦". iMod ("ToBor" with "[↦ Pc]") as "[? κ]".
     { iNext. iExists _, _. iFrame "⧖ Pc". iExists _. by iFrame. }
     iMod ("ToL" with "κ") as "$". iFrame "In". iExists _, _. by iFrame.
-  Qed.
-
-  Lemma tctx_reborrow_uniq {𝔄} E L p (ty: type 𝔄) κ κ' :
-    lctx_lft_incl E L κ' κ →
-    tctx_incl E L +[p ◁ &uniq{κ} ty] +[p ◁ &uniq{κ'} ty; p ◁{κ'} &uniq{κ} ty]
-      (λ post '-[(a, a')], ∀a'': 𝔄, post -[(a, a''); (a'', a')]).
-  Proof.
-    intros κκ'. split; [intros ??? [[??][]]; by apply forall_proper|].
-    iIntros (??[vπ[]]?) "#LFT #PROPH #UNIQ E L [p _] Obs".
-    have ?: Inhabited 𝔄 := populate (vπ inhabitant).1.
-    iDestruct (κκ' with "L E") as "#κ⊑κ'". iFrame "L".
-    iDestruct "p" as ([[]|]??) "[⧖ [#In uniq]]"=>//.
-    iDestruct "uniq" as (? ξi [Le Eq]) "[ξVo ξBor]". set ξ := PrVar _ ξi.
-    move: Le=> /succ_le[?[->?]].
-    iMod (rebor with "LFT κ⊑κ' ξBor") as "[ξBor ToξBor]"; [done|].
-    iMod (uniq_intro (fst ∘ vπ) with "PROPH UNIQ") as (ζi) "(ζVo & ζPc)"; [done|].
-    set ζ := PrVar _ ζi.
-    iMod (bor_create _ κ' (∃vπ' d', .VO[ξ] vπ' d' ∗ ⧖(S d') ∗ .PC[ζ] vπ' d')%I
-      with "LFT [⧖ ξVo ζPc]") as "[ζBor ToζBig]"; [done| |].
-    { iExists _, _. iFrame "ξVo ζPc". iApply persistent_time_receipt_mono; [|done]. lia. }
-    iMod (bor_combine with "LFT ξBor ζBor") as "Bor"; [done|].
-    iExists -[λ π, ((vπ π).1, π ζ); λ π, (π ζ, (vπ π).2)]. iSplitR "Obs"; last first.
-    { iApply (proph_obs_impl with "Obs") => /= π. case (vπ π)=>/= ?? All. apply All. }
-    iMod (bor_acc_atomic_cons with "LFT Bor") as
-      "[[[ξBig ζBig] ToBor]|[#†κ' TolftN]]"; [done| |]; last first.
-    { iMod "TolftN" as "_". iMod ("ToξBor" with "†κ'").
-      iMod ("ToζBig" with "†κ'") as (??) "(>ξVo & >#⧖ & ζPc)".
-      iMod (uniq_strip_later with "ζVo ζPc") as (<-<-) "[ζVo ζPc]". iSplitL "ζVo".
-      - iExists _, _. iFrame "⧖". iSplitR; [done|].
-        iSplitR; [by iApply lft_incl_trans|]. iExists _, ζi. iFrame "ζVo".
-        iSplitR; [done|]. by iApply bor_fake.
-      - iModIntro. iSplitL; [|done]. iExists _. iSplit; [done|]. iIntros "_!>".
-        iExists _, _. iFrame "⧖". iSplitL "ζPc"; last first.
-        { iFrame "In". iExists _, _. by iFrame. }
-        iNext. iDestruct (proph_ctrl_eqz with "PROPH ζPc") as "Eqz".
-        iApply (proph_eqz_pair with "[Eqz]"); [done|iApply proph_eqz_refl]. }
-    iDestruct "ξBig" as (??) "(>#⧖ & ξPc & ↦ty)".
-    iDestruct "ζBig" as (??) "(>ξVo & _ & ζPc)".
-    iMod (uniq_strip_later with "ξVo ξPc") as (<-<-) "[ξVo ξPc]".
-    iMod (uniq_strip_later with "ζVo ζPc") as (<-<-) "[ζVo ζPc]".
-    iMod ("ToBor" $! (∃ vπ' d', ⧖(S d') ∗ .PC[ζ] vπ' d' ∗
-      l ↦∗: ty.(ty_own) vπ' d' tid)%I with "[ξVo ξPc] [ζPc ↦ty]") as "ζBor".
-    { iIntros "!> (%&% & #? & ζPc & ↦ty)".
-      iMod (uniq_update with "UNIQ ξVo ξPc") as "[ξVo ξPc]"; [solve_ndisj|].
-      iSplitL "↦ty ξPc"; iExists _, _; by iFrame. }
-    { iNext. iExists _, _. by iFrame. }
-    iModIntro. iSplitL "ζVo ζBor"; [|iSplitL; [|done]].
-    { iExists _, _. iSplit; [done|]. iFrame "⧖".
-      iSplitR; [by iApply lft_incl_trans|]. iExists _, _. by iFrame. }
-    iExists _. iSplit; [done|]. iIntros "#†κ'". iMod ("ToξBor" with "†κ'") as "ξBor".
-    iMod ("ToζBig" with "†κ'") as (vπ' ?) "(>ξVo & >⧖' & ζPc)". iModIntro.
-    iExists _, _. iFrame "⧖' In". iSplitL "ζPc".
-    - iNext. iDestruct (proph_ctrl_eqz with "PROPH ζPc") as "Eqz".
-      iApply (proph_eqz_pair _ (pair ∘ vπ' ⊛ (snd ∘ vπ)) with "[Eqz]");
-      [done|iApply proph_eqz_refl].
-    - iExists _, _. rewrite (proof_irrel (prval_to_inh' _) (prval_to_inh' vπ)).
-      by iFrame.
-  Qed.
-
-  Lemma tctx_extract_hasty_reborrow {𝔄 𝔅l} (ty ty': type 𝔄) κ κ' (T: tctx 𝔅l) E L p :
-    lctx_lft_incl E L κ' κ → eqtype E L ty ty' id id →
-    tctx_extract_elt E L (p ◁ &uniq{κ'} ty) (p ◁ &uniq{κ} ty' +:: T)
-      (p ◁{κ'} &uniq{κ} ty' +:: T) (λ post '((a, a') -:: bl),
-        ∀a'': 𝔄, post ((a, a'') -:: (a'', a') -:: bl)).
-  Proof.
-    move=> ??. eapply tctx_incl_impl.
-    - apply (tctx_incl_frame_r +[_] +[_;_]).
-      eapply tctx_incl_trans; [by apply tctx_reborrow_uniq|].
-      by apply subtype_tctx_incl, uniq_subtype, eqtype_symm.
-    - by move=>/= ?[[??]?].
-    - intros ??? [[??]?]. by apply forall_proper.
   Qed.
 
   Lemma tctx_uniq_mod_ty_out {𝔄 𝔅 ℭl} κ f ty (T: tctx ℭl) p E L
@@ -406,5 +292,4 @@ Global Hint Extern 0 (typed_write _ _ (&uniq{_} _) _ _ _ _ _) =>
 Global Hint Extern 0 (typed_read _ _ (&uniq{_} _) _ _ _ _) =>
   simple apply read_uniq : lrust_typing.
 
-Global Hint Resolve tctx_extract_hasty_reborrow | 10 : lrust_typing.
 Global Hint Resolve tctx_extract_uniq_eqtype | 5 : lrust_typing.
