theories/typing/type.v
@@ -1118,15 +1118,6 @@ End subtyping.
 Section type_util.
   Context `{!typeG Σ}.
 
-  Lemma heap_mapsto_ty_own {𝔄} l (ty: type 𝔄) vπ d tid :
-    l ↦∗: ty.(ty_own) vπ d tid ⊣⊢
-    ∃vl: vec val ty.(ty_size), l ↦∗ vl ∗ ty.(ty_own) vπ d tid vl.
-  Proof.
-    iSplit; iIntros "[%vl[? ty]]"; [|iExists vl; by iFrame].
-    iDestruct (ty_size_eq with "ty") as %<-. iExists (list_to_vec vl).
-    rewrite vec_to_list_to_vec. iFrame.
-  Qed.
-
   Definition by_succ (d: nat) (Φ: nat → iProp Σ) : iProp Σ :=
     match d with S d' => Φ d' | _ => False end.
   Lemma by_succ_ex d Φ : by_succ d Φ ⊣⊢ ∃d', ⌜d = S d'⌝ ∗ Φ d'.
@@ -1173,6 +1164,31 @@ Notation "[S( d' ) := d ] P" := (by_succ d (λ d', P)) (at level 200,
 
 Notation "[loc[ l ] := vl ] P" := (by_just_loc vl (λ l, P)) (at level 200,
   right associativity, format "[loc[ l ]  :=  vl ]  P") : bi_scope.
+
+Section type_util.
+  Context `{!typeG Σ}.
+
+  (* Splitting for a standard pointer *)
+  Lemma split_mt_ptr Φ d l' :
+    (l' ↦∗: λ vl, [S(d') := d] [loc[l] := vl] Φ d' l) ⊣⊢
+    [S(d') := d] ∃l: loc, l' ↦ #l ∗ Φ d' l.
+  Proof.
+    iSplit.
+    - iIntros "(%vl & ↦ &?)". case d as [|]=>//. case vl as [|[[]|][]]=>//.
+      rewrite heap_mapsto_vec_singleton. iExists _. iFrame.
+    - iIntros "big". case d as [|]=>//. iDestruct "big" as (?) "[??]".
+      iExists [_]. rewrite heap_mapsto_vec_singleton. by iFrame.
+  Qed.
+
+  Lemma heap_mapsto_ty_own {𝔄} l (ty: type 𝔄) vπ d tid :
+    l ↦∗: ty.(ty_own) vπ d tid ⊣⊢
+    ∃vl: vec val ty.(ty_size), l ↦∗ vl ∗ ty.(ty_own) vπ d tid vl.
+  Proof.
+    iSplit; iIntros "[%vl[? ty]]"; [|iExists vl; by iFrame].
+    iDestruct (ty_size_eq with "ty") as %<-. iExists (list_to_vec vl).
+    rewrite vec_to_list_to_vec. iFrame.
+  Qed.
+End type_util.
 
 Global Hint Resolve ty_outlives_E_elctx_sat tyl_outlives_E_elctx_sat : lrust_typing.
 Global Hint Resolve leak'_post | 5 : lrust_typing.
